<?xml version="1.0" encoding="UTF-8"?>

<section xml:id="subsec-3-5-proofs-of-or" xmlns:xi="http://www.w3.org/2001/XInclude">
<title>Proofs with Conjunctions and Disjunctions</title>
    <p>
        So far we have been proving the prototypical 
        <me>
            P\implies Q
        </me>
        as it is perhaps one of the most common propositional forms used in mathematics, and otherwise. 
        Yet, in all of our examples thus far both <m>P</m> and <m>Q</m> have been atomic propositions. In this 
        section we will be substituting the antecedent and consequent with compound propositions. 
    </p>
    <assemblage>
        <title>Assuming an Or</title>
        <idx><h>disjunction</h><h>proofs with assuming or</h></idx>
        <idx><h>or</h><h>proofs with assuming or</h></idx>
        <p>
          For propositions <m>P</m>, <m>Q</m>, and <m>R</m>, to prove a statement in the form of 
          <me>
            (P\vee R)\implies Q
          </me>
          
        </p>
        <p>
            First we:
        </p>
        <p>
            <alert>Prove:</alert> <m>P\implies Q</m>
        </p>
        <p>
            then we:
        </p>
        <p>
            <alert>Prove:</alert> <m>R\implies Q</m>
        </p>
      </assemblage>
      <p>
        To verify that this argument is valid, we will use a truth table to show:
        <me>
            [(P\implies Q)\wedge(R\implies Q)]\implies [(P\vee R)\implies Q]
        </me>
        is a tautology. To do so we will show a stronger result using the tricks of <xref ref="subsec-2-4-3-logic-algebra"/>.
      </p>
      <md>
        <mrow>(P\vee R)\implies Q\amp \equiv [\sim (P\vee R)]\vee Q \text{ (Rob's Law)}</mrow>
        <mrow>\amp \equiv [(\sim P)\wedge (\sim R)]\vee Q \text{ (De Morgan's)}</mrow>
        <mrow>\amp \equiv [(\sim P)\vee Q]\wedge[ (\sim R)\vee Q ]\text{ (distribution)}</mrow>
        <mrow>\amp \equiv [P\implies Q]\wedge[R\implies Q] \text{ (Rob's Law)}</mrow>
    </md>
      <p>
        Now lets see an example of this in play.
      </p>
      <example>
        <p>
            <alert>Prove:</alert> for any two integers <m>x</m> and <m>y</m> if <m>x</m> is even or <m>y</m>
            is even then <m>x\cdot y</m> is even.
        </p>
       <proof>
       <p>
        Let <m>x</m> and <m>y</m> be integers.</p> 
        <p>
        First assume that <m>x</m> is even. By definition of even 
        (<xref ref="defn-even"/>) we can find an integer <m>k</m> so that <m>x=2k</m>. Calculate:
        <md>
            <mrow>x\cdot y\amp=(2k)\cdot y</mrow>
            <mrow>\amp=2(ky)</mrow>
        </md>
        since <m>ky</m> is an integer by the definition of even, <m>x\cdot y</m> is even.
       </p>
       <p>
        Next, we instead assume <m>y</m> is even. By definition of even we can find an integer <m>t</m>
        so that <m>y=2t</m>. Calculate:
        <md>
            <mrow>x\cdot y\amp=x\cdot(2t)</mrow>
            <mrow>\amp=2(xt)</mrow>
        </md>
        since <m>xt</m> is an integer by the definition of even, <m>x\cdot y</m> is even.
       </p>
       <p>
        Now since we have shown that for <m>\forall x,y\in\Z</m> that both <m>x</m> is even implies <m>x\cdot y</m>
        is even and <m>y</m> is even implies <m>x\cdot y</m> is even,
        we have shown that <m>\forall x,y\in\Z</m>.
       </p>
    </proof>
      </example>
      <p>
        Another interesting scenario is when we are trying to conclude a disjunction.
      </p>
      <assemblage>
        <title>Concluding an Or</title>
        <idx><h>disjunction</h><h>concluding or</h></idx>
        <idx><h>or</h><h>concluding or</h></idx>
        <p>
          For propositions <m>P</m>, <m>Q</m>, and <m>R</m>, to prove a statement in the form of 
          <me>
            P\implies (Q\vee R)
          </me>
          
        </p>
        <p>
            We instead 
        </p>
        <p>
            <alert>Prove:</alert> <m>[P\wedge(\sim R)]\implies Q</m>
        </p>
        
      </assemblage>
      <p>
        That this argument is valid can be seen by showing that 
        <me>
            [P\implies(Q\vee R)]\equiv[[P\wedge(\sim R)]\implies Q]
        </me>
        To do that we will again use the tricks of <xref ref="subsec-2-4-3-logic-algebra"/>.
      </p>
      <p>
      <md>
        <mrow>P\implies (Q\vee R)\amp \equiv (\sim P)\vee( Q\vee R) \text{ (Rob's Law)}</mrow>
        <mrow>\amp \equiv (\sim P)\vee (R\vee Q) \text{ (commutativity)}</mrow>
        <mrow>\amp \equiv [(\sim P)\vee R]\vee Q \text{ (associativity)}</mrow>
        <mrow>\amp \equiv \sim[P\wedge (\sim R)]\vee Q \text{ (De Morgan's)}</mrow>
        <mrow>\amp \equiv (P\wedge (\sim R))\implies Q \text{ (Rob's Law)}</mrow>
    </md>
    </p>
    <p>
    Now lets see an example.
    </p>
    <example>
        <p>
            <alert>Prove:</alert> For all integers <m>x</m> and <m>y</m> if <m>x</m> is even then
            <m>y</m> is odd or <m>x+y</m> is even
        </p>
       <proof>
        <p>
            Let <m>x</m> and <m>y</m> be arbitrary integers. Assume that <m>x</m> is even and that 
            <m>y</m> is not odd. By the definition of even (<xref ref="defn-even"/>) we can find
            an integer <m>k</m> so that <m>x=2k</m>. By the division algorithm
            (<xref ref="sec-4-1-1-what-we-assume"/>) we can find integers <m>q</m> and <m>r</m> such that 
            <m>0\leq r\lt 2</m> such that <m>y=2q+r</m>. Yet since we assumed <m>y</m> is not odd <m>r\neq 1</m>, 
            and since <m>r</m> is an integer and <m>0\leq r\lt 2</m> and the only integers which satisfy this inequality
            are 0 and 1, which only leaves <m>r=0</m> thus <m>y=2q</m>. 
            Now calculate:
            <md>
                <mrow>x+y\amp=2k+2q</mrow>
                <mrow>\amp=2(k+q)</mrow>
            </md>
            Since <m>k+q</m> is an integer by the definition of even <m>x+y</m> is even. 
        </p>
        <p>
            Since we have assumed for two arbitrary integers <m>x</m> and <m>y</m> that <m>x</m> is even and <m>y</m> is 
            not odd, and we have concluded that <m>x+y</m> is even, we can conclude that for all integers <m>x</m> and <m>y</m>, if <m>x</m> is even then
            <m>y</m> is odd or <m>x+y</m> is even.
        </p>
        </proof>
    </example>
    <p>
      The last propositional form we consider in this section is the following.
    </p>

    <assemblage>
      <title>Concluding an And</title>
      <idx><h>conjunction</h><h>concluding an and</h></idx>
      <idx><h>and</h><h>concluding an and</h></idx>
      <p>
        For propositions <m>P</m>, <m>Q</m>, and <m>R</m>, one way to prove a statment in the form of 
        <me>
          P\implies (Q\wedge R)
        </me>
        
      </p>
      <p>
          First we:
      </p>
      <p>
          <alert>Prove:</alert> <m>P\implies Q</m>
      </p>
      <p>
          then we:
      </p>
      <p>
          <alert>Prove:</alert> <m>P\implies R</m>
      </p>
    </assemblage>
    <p>
      To see that this is a valid way of proving, we once again show an even stronger 
      result using the methods of <xref ref="subsec-2-4-3-logic-algebra"/>.
    </p>
    <p>
    <md>
      <mrow>P\implies (Q\wedge R)\amp \equiv (\sim P)\vee( Q\wedge R) \text{ (Rob's Law)}</mrow>
      <mrow>\amp \equiv [(\sim P)\vee Q]\wedge [(\sim P)\vee R] \text{ (distribution)}</mrow>
      <mrow>\amp \equiv [P\implies Q]\wedge [P\implies R] \text{ (Rob's Law)}</mrow>
  </md>
  </p>
   
    <example>
      <p>
        <alert>Prove:</alert> For all integers <m>a</m> and <m>b</m>, if <m>3|(a-2)</m> and <m>3|(b-1)</m> then <m>3|(a+b)</m> and <m>3|(a-2b)</m>
      </p>
      <proof>
      
        <p>
          Let <m>a</m> and <m>b</m> be arbitrary integers. 
        </p>
        <p>
          Assume that <m>3|(a-2)</m>, also assume that <m>3|(b-1)</m>. By definition of divides (<xref ref="defn-divides"/>) we can produce an 
          integer <m>k</m> such that <m>a-2=3k</m>, and hence by adding 2 to both sides of this equation we get
          <m>a=3k+2</m>. As well by the definition of divides we can come forth with another integer <m>t</m> with the 
          property that <m>b-1=3t</m>, this time adding 1 to both sides of the equation we see that <m>b=3t+1</m>.
        </p>
        <p>
          Now, we will prove: if <m>3|(a-2)</m> and <m>3|(b-1)</m> then <m>3|(a+b)</m>, by calculating:
          <md>
            <mrow>a+b\amp=(3k+2)+(3t+1)</mrow>
            <mrow>\amp=3k+3t+3</mrow>
            <mrow>\amp=3(k+t+1)</mrow>
        </md>
        and since <m>k+t+1</m> is an integer by the definition of divides <m>3|(a+b)</m>.
        </p>
        
        <p>
          Next, we will prove: if <m>3|(a-2)</m> and <m>3|(b-1)</m> then <m>3|(a-2b)</m>, instead by calculating:
          <md>
            <mrow>a+b\amp=(3k+2)-2(3t+1)</mrow>
            <mrow>\amp=3k+2-6t-2</mrow>
            <mrow>\amp=3k-6t</mrow>
            <mrow>\amp=3(k-2t)</mrow>
        </md>
        and since <m>k-2t</m> is an integer by the definition of divides <m>3|(a-2b)</m>.
        </p>
        <p>
          Now that we have assumed that <m>a</m> and <m>b</m> are arbitrary integers and assumed that <m>3|(a-2)</m> and <m>3|(b-1)</m> 
          then we showed that both <m>3|(a+b)</m> and that <m>3|(a-2b)</m> we can conclude that for all integers <m>a</m> and <m>b</m>, 
          if <m>3|(a-2)</m> and <m>3|(b-1)</m> then <m>3|(a+b)</m> and <m>3|(a-2b)</m>.
        </p>

        
      </proof>
    </example>
</section>