<?xml version="1.0" encoding="UTF-8"?>

<section xml:id="sec-6-4-fib" xmlns:xi="http://www.w3.org/2001/XInclude">
  <title>The Fibonacci Sequence</title>
  <p>
    blah... wax poetic about defining someting inductively... blah... that means cleaning up the below definiton.. blah... also don't forget the bunny story... blah..
  </p>
   <assemblage>
        <title>Fibonacci numbers</title>
        <p>
            To calculate any Fibonacci number, <m>f_n</m>, we add the two numbers that preceded it: 
        <me>
            f_n = f_{n-1} + f_{n-2}
        </me>
        </p>
        <p>
           where <m>f_1=1</m> and <m>f_2=1</m>
        </p>
    </assemblage>
    <p>
      blah.. some examples of calculating this would be nice!.. blah...
    </p>
    <assemblage>
    <title>Priciple of Complete Induction</title>

    <p>
        Let <m>k\in\N</m> and suppose <m>S</m> is a subset of <m>\mathbb{N}</m> with the following property:
    </p>
    <p>
        <m>\forall n\in \mathbb{N}</m> with <m>k\lt n</m> 
    </p>
    <p>
        if <m>\{k,k+1,k+2,k+3,...,n-1\} \subset S</m> then <m>n \in S</m>
    </p>
    <p>
        Then <m>S=\{n\in\N\text{ }|\text{ }n\geq k\}</m> 
    </p>
  </assemblage>
  <p>
    Proving using complete induction amounts to a procedure almost identical to that of our traditional induction
  </p>
  <assemblage>
    <title>Proof of <m>\forall m\in\N</m> <m>m\geq k</m> <m>P(m)</m> with Complete Induction</title>
    <p>
      Proof:
      <ol marker="(i)">
        <li>
          <p>
            <alert>(Base Step)</alert> Show that <m>P(k)</m> is true
          </p>
        </li>
        <li>
          <p>
            <alert>(Induction Assumption)</alert> Assume we can find an <m>n\in\N</m> such that <m>P(t)</m> is true for any <m>t\in\N</m> such that <m>k\leq t\lt n</m>
          </p>
        </li>
        <li>
          <p>
            <alert><m>\mathbf{\left(\text{Prove: }P(n)\right)}</m></alert> ... thus <m>P(n)</m> is true
          </p>
        </li>
      </ol>
      Therefore <m>\forall m\in\N</m> such that <m>m\geq k</m> then <m>P(m)</m> is true.
    </p>
  </assemblage>
  <p>
    The astute student will note we are really doing nothing different here... as in PMI we said <em>for any</em> <m>n</m> so why not <m>n-1</m>. But, this really allows us to do exactly what we have been doing its just that in step (iii) it becomes quite cumbersome to balance <m>n+1</m> everywhere, so this way just lets us use <m>n</m>.
  </p>
    <example>
      <p>
            <alert>Prove:</alert> For any <m>m\in\N</m> such that <m>m\geq 1</m> we have <m>f_{3m}</m> is even (every third fibonacci number is even)
        </p>
      <proof>
        
        <p>
            <alert>(i) (Base Case):</alert> 
        </p>
        <p>
            As we are to show this result for any <m>m\geq 1</m>, our base case will be 1!
            <me>
                f_{3\cdot 1}=f_2+f_1=1+1=2
            </me>
            and since 1 is an integer and thus <m>2=2\cdot 1</m> is even and hence we have established the base case:
            <me>
                P(1): f_{3\cdot(1)}\text{ is even}
            </me>
            
        </p>
        <p>
            <alert>(ii) (Induction Assumption):</alert>
        </p>
        <p>
            Assume we can find an <m>n\in\N</m> such that 
            <me>
                f_{3t} \text{ is even}
            </me>
            for any <m>t\in\N</m> such that <m>1\leq t\lt n</m>
        </p>
        <p>
            <alert>(iii) <m>\mathbf{\left(\text{Prove: }P(n)\right)}</m></alert>
        </p>
        <p>
            Calculate:
        </p>
        <md>
            <mrow>f_{3n}\amp=f_{3n-1}+f_{3n-2}</mrow>
            <mrow> \amp=f_{3n-2}+f_{3n-3}+f_{3n-2}</mrow>
            <mrow> \amp=2(f_{3n-2})+f_{3(n-1)}</mrow>
        </md>
        <p>
            Hence, by induction assumption, <m>f_{3(n-1)}</m> is even. Thus by definition of even, we can find an integer <m>m</m> such that <m>f_{3(n-1)}=2m</m>
        </p>
        <p>
            Calculate:
        </p>
        <md>
            <mrow>f_{3n}\amp=2f_{3n-2}+2m</mrow>
            <mrow> \amp=2(f_{3n-2+m})</mrow>
        </md>
        <p>
            Thus by definition of even, <m>f_{3n}</m> is even. Thus by proof by PCI, <m>f_{3n}</m> is even for all <m>n\in \mathbb{N}</m>
        </p>
    </proof>

    </example>
    <p>
      blah..
    </p>
    <example>
      <p>
        
            <alert>Prove:</alert> For any <m>m\in\N</m> such that <m>m\geq 1</m> we have <m>f_{3m+1}</m> is odd 
        
      </p>
      <proof>
        
        <p>
            <alert>(i) (Base Case):</alert> 
        </p> 
        <p>
            Since, again, we are to show this for any <m>m\geq 1</m>, our base case is 1!
            <me>
                f_{3(1)+1}=f_4=f_3+f_2=(f_2+f_1)+f_2=(1+1)+1=3
            </me>
            Since 1 is an integer and <m>3=1\cdot(1)+1</m> we have that 3 is odd. Hence, we have estableshed the base case 
            <me>
                P(1):f_{3\cdot(1)+1}\text{ is odd}
            </me>
            
        </p>
        <p>
            <alert>(ii) (Induction Assumption):</alert>
        </p>
        <p>
            Assume we can find an <m>n\in\N</m> such that 
            <me>
                f_{3t+1} \text{ is odd}
            </me>
            for any <m>t\in\N</m> such that <m>1\leq t\lt n</m>
        </p>
        <p>
            <alert>(iii) <m>\mathbf{\left(\text{Prove: }P(n)\right)}</m></alert>
        </p>
        <p>
            Calculate:
        </p>
        <md>
            <mrow>f_{3n+1}\amp=f_{3n}+f_{3n-1}</mrow>
            <mrow> \amp=f_{3n}+f_{3n-2}+f_{3n-3}</mrow>
            <mrow> \amp=2(f_{3n})+f_{3n-2}+f_{3(n-1)}</mrow>
            <mrow> \amp=2(f_{3n})+f_{3(n-1)+1}+f_{3(n-1)}</mrow>
        </md>
        <p>
            Note: we know <m>f_{3n}</m> and <m>f_{3(n-1)}</m> are even, because we just proved it. By our induction assumption, <m>f_{3(n-1)+1}</m>
            is odd. Hence by definition of odd, we can find <m>l,m,a\in \mathbb{Z}</m> such that <m>f_{3n}=2l</m>, <m>f_{3(n-1)}=2m</m>, and
            <m>f_{3(n-1)+1}=2a+1</m>.
        </p>
        <p>
            Calculate:
        </p>
        <md>
            <mrow>f_{3n}+f_{3(n-1)+1}+f_{3(n-1)}\amp=2l+2a+1+2m</mrow>
            <mrow> \amp=2(l+a+m)+1</mrow>
        </md>
        <p>
            Thus by definition of odd, <m>f_{3n+1}</m> is odd. Thus by proof by PCI, <m>f_{3n+1}</m> is odd for all <m>n\in \mathbb{N}</m>
        </p>
    </proof>
    </example>
</section>