<?xml version="1.0" encoding="UTF-8"?>

<section xml:id="sec-6-6-exercises" xmlns:xi="http://www.w3.org/2001/XInclude">
  <title>Exercises</title>
  <p>
    
   
    <ol>
      <li>
        <p>
           Use Induction to prove that the following hold
          <ol>
        <li>
            <p>
                <m>\displaystyle \sum_{i=1}^{n} 2^i = 2^{n+1} - 2</m> for all <m>m\geq 1</m>
            </p>
        </li>
        <li>
            <p>
                <m>\displaystyle\sum_{i=1}^{n} (2i-1)^3 = n^2(2n^2-1)</m> for all <m>m\geq 1</m>
            </p>
        </li>
        <li>
            <p>
                <m>\displaystyle\prod_{i=1}^{n}(2i-1) = \frac{(2n)!}{n!2^n}</m> for all <m>m\geq 1</m>
            </p>
        </li>
        <li>
          <p>
            <m>\displaystyle \sum_{i=1}^{m} (3i-2) = \frac{m}{2}(3m-1)</m> for all <m>m\geq 1</m>
          </p>
        </li>
        <li>
          <p>
            <m>\displaystyle \sum_{i=1}^m (2i-1)^3=m^2(2m^2-1)</m> for all <m>m\geq 1</m>
          </p>
        </li>
        <li>
          <p>
            <m>\displaystyle \sum_{i=1}^m \frac{i}{(i+1)!}=1-\frac{1}{(m+1)!}</m>
          </p>
        </li>
        <li>
          <p>
            <m>\displaystyle \sum_{i=0}^{m}3^i=\frac{3^{m+1}-1}{2}</m> for all <m>m\in\N</m>
          </p>
        </li>
        <li>
            <p>
                <m>f_1 + f_2 + f_3 + ... + f_m = f_{m+2}-1</m> for all <m>m\geq 1</m>
            </p>
        </li>
        <li>
          <p>
            <m>f_{m+6}=4f_{m+3}+f_m</m> for all <m>m\geq 1</m>
          </p>
        </li>
        <li>
          <p>
            <m>f_{3m+2}</m> is odd for all <m>m\geq 1</m>
          </p>
        </li>
        
    </ol>
        </p>
      </li>
      <li>
        <p>
          Let <m>\mathscr{A}=\{A_i\text{ }|\text{ }i\leq m\}</m> be an indexed family of sets, prove: <m>\displaystyle \left(\bigcup_{i=1}^m a_i\right)^c=\bigcap_{i=1}^m A_i^c</m> for all <m>m\geq 1</m>
        </p>
      </li>
    </ol>

  </p>

</section>