<?xml version="1.0" encoding="UTF-8"?>

<section xml:id="sec-10-4" xmlns:xi="http://www.w3.org/2001/XInclude">
  <title>Partitions, bijections, etc.</title>
  <p>
    This is starting from week 13 in my notes...
  </p>
  
  <definition xml:id="def-partition">
    <title>Partition</title>
    <statement>
      <p>
        Let <m>A</m> be a non-empty set. <m>\mathscr{P}</m> is a partition of <m>A</m> if <m>\mathscr{P}</m> is a set of subsets of <m>A</m>
        such that:
      </p>
      <ol marker="i.)">
        <li>
          <p>
            If <m>X\in \mathscr{P} \text{, then }x\neq \emptyset</m>
          </p>
        </li>
        <li>
          <p>
            If <m>X\in \mathscr{P}</m> and <m>Y \in \mathscr{P}</m>, then <m>x=y \text{ or }x\cap y = \emptyset</m>
          </p>
        </li>
        <li>
          <p>
            <m>\cup X = A</m> for all <m>x\in \mathscr{P}</m>
          </p>
        </li>
      </ol>
    </statement>
  </definition>
  
  <definition xml:id="def-function">
    <title>Function</title>
    <statement>
      <p>
        A function, or mapping, from <m>A</m> to <m>B</m> is a relation <m>f</m> from <m>A</m> to <m>B</m> such that:
      </p>
      <ol marker="i.)">
        <li>
          <p>
            The domain of <m>f</m> is <m>A</m>.
          </p>
        </li>
        <li>
          <p>
            If <m>(x,y)\in f</m> and <m>(x,z)\in f</m> then <m>y=z</m>
          </p>
        </li>
      </ol>
      <p>
        We write <m>f: A \rightarrow B</m>. We <em>say</em> "<m>f</m> is a function from <m>A</m> to <m>B</m>,"
        or "<m>f</m> maps <m>A</m> to <m>B</m>."
      </p>
      <p>
        The set <m>B</m> is called the codomain of <m>f</m>. In the case where <m>B=A</m>, we say that "<m>f</m> is a function
        on <m>A</m>."
      </p>
      <p>
        When <m>(x,y)\in f</m>, we write <m>y=f(x)</m>, and we say that <m>y</m> is the image of <m>f</m> at <m>x</m>,
        and that <m>x</m> is a pre-image of <m>y</m>.
      </p>
    </statement>
  </definition>

  <definition xml:id="def-surjection">
    <title>Surjection</title>
    <statement>
      <p>
        A function <m>f:A \rightarrow B</m> is <em>onto</em> <m>B</m>, or is a <term>surjection</term> if
        Rng<m>(f)=B</m>. When <m>f</m> is a surjection, we write <m>f:A \twoheadrightarrow B</m> or 
        <m>f: A \overset{\text{onto}}{\rightarrow} B</m>.
      </p>
    </statement>
  </definition>

  <definition xml:id="def-injection">
    <title>Injection</title>
    <statement>
      <p>
        A function <m>f:A \rightarrow B</m> is one-to-one, or is an <term>injection</term>, if whenever <m>f(x)=f(y)</m>
        then <m>x=y</m>. We write this as <m>f:A \hookrightarrow B</m>, or <m>f: A \overset{\text{1-1}}{\rightarrow} B</m>.
      </p>
    </statement>
  </definition>

  <definition xml:id="def-bijection">
    <title>Bijection</title>
    <statement>
      <p>
        A function <m>f:A \rightarrow B</m> is a one-to-one correspondence, or a <term>bijection</term> if <m>f</m>
        is one-to-one and onto <m>B</m>. We write this as <m>f: A \overset{\sim}{\rightarrow} B</m>
      </p>
    </statement>
  </definition>

<section>
  <p>
    Consider the set <m>A = \{a, b, c, d, e\}</m>, and the family <m>C = \{C_1, C_2, C_3\}</m> where <m>C_1 = \{b,e\}</m>,
    <m>C_2 = \{a,c,d\}</m>, and <m>C_3 = \{b,e\}</m>
  </p>
  <p>
    It passes all three tests, so the family <m>C</m> is a partition of <m>A</m>, even thought the sets <m>C_1</m>
    and <m>C_3</m> are not disjoint.
  </p>
  <p>
    The family <m>\{C_1, C_2, C_3\}</m> is the same as the family <m>\{C_2, C_3</m>.
  </p>

  <theorem xml:id="thm-10-4-1">
    <statement>
      <p>
        If <m>R</m> is an equivalence relation on a non-empty set <m>A</m> then <m>A/R</m> is a partition of <m>A</m>.
      </p>
    </statement>
  </theorem>

  <theorem xml:id="thm-10-4-2">
    <statement>
      <p>
        Let <m>\mathscr{P}</m> be a partition of the nonempty set <m>A</m>. For <m>x</m> and <m>y\in A</m> define <m>xQy</m> if and
        only if there exists <m>C\in \mathscr{P}</m> such that <m>x\in C</m> and <m>y\in C</m>. Then <m>Q</m> is an equivalence
        relation on <m>A</m>.
      </p>
      
    </statement>
  </theorem>

  <proof>
    <p>
      <alert>[Reflexive]</alert>
    </p>
    <p>
      let <m>x\in A</m>. Since <m>\mathscr{P}</m> is a partition, <m>x\in \cup X = A</m>. Hence we can find a <m>C \in \mathscr{P}</m>
      such that <m>x\in C</m>. Hence, <m>(x,x)\in Q</m>, since <m>x\in C</m>.
    </p>
    <p>
      <alert>[Symmetric]</alert>
    </p>
    <p>
      Let <m>(x,y)\in Q</m>. By definition of <m>Q</m> we can find <m>C\in \mathscr{P}</m> such that <m>x\in C</m> and 
      <m>y\in C</m>. Hence, <m>y\in C</m> and <m>x\in C</m>. Thus by definition of <m>Q, (y,x)\in Q</m>.
    </p>
    <p>
      <alert>[Transitive]</alert>
    </p>
    <p>
      Let <m>(x,y)\in Q</m> and <m>(y,z)\in Q</m>. By definition of <m>Q</m> we can find <m>C_1, C_2 \in \mathscr{P}</m>
      such that <m>x\in C_1</m> and <m>y\in C_1</m>, and <m>y\in C_2</m> and <m>z\in C_2</m>. Hence, <m>y\in C_1 \cap C_2</m>.
      Hence <m>C_1\cap C_2 \neq \emptyset</m>. Hence by definition of partition, <m>C_1=C_2</m>. Hence <m>x\in C</m>
      and <m>z\in C</m>. Hence by definition of <m>Q, (x,z) \in Q</m>. 
    </p>
  </proof>
  
  <p>
    <alert>Prove:</alert> If <m>f: A \rightarrow B</m> is one-to-one and <m>g: B \rightarrow C</m> is one-to-one, then 
    <m>g\circ f</m> is one-to-one.
  </p>

  <proof>
    <p>
      Assume <m>f: A \hookrightarrow B</m> and <m>g: B \hookrightarrow C</m>. Let <m>(x,y)\in A</m> such that 
      <m>g\circ f(x) = g\circ f(y)</m>.
    </p>
    <p>
      By definition of composition we can find <m>z\in B</m> such that <m>f(x) = z</m> and <m>g(z) = g\circ f(x)</m>.
      Also by definition of composition, we can find <m>w\in B</m> such that <m>f(y) = w</m> and <m>g(w) = g\circ f(y)</m>.
    </p>
    <p>
      By assumption that <m>g\circ f(x) = g\circ f(y), g(w) = g(z)</m>. By our assumption that <m>g</m> is one-to-one, <m>w=z</m>.
      Since <m>w=z, f(x)=f(y)</m>. Thus, by our assumption that <m>f</m> is one-to-one, <m>x=y</m>.
    </p>
  </proof>

  <theorem xml:id="thm-10-4-3">
    <statement>
      <p>
        If <m>f: A\rightarrow B</m> is a bijection, and <m>g: B\rightarrow C</m> is a bijection, then <m>g\circ f: A\rightarrow C</m>
        is a bijection.
      </p>
    </statement>
  </theorem>

  <proof>
    <p>
      Assume <m>f</m> is a bijection from <m>A</m> to <m>B</m> and <m>g</m> is a bijection from <m>B</m> to <m>C</m>.
    </p>
    <p>
      <alert>[1-to-1]</alert>
    </p>
    <p>
      Let <m>x\in A</m> and <m>y\in A</m> such that <m>g\circ f(x) = g\circ f(y)</m>. By definition of composition we can find
      <m>z\in B</m> and <m>w\in B</m> such that <m>g(w) = g\circ f(y)</m> and <m>f(y) = w</m> and <m>g(z) = g\circ f(x)</m> 
      and <m>f(x) = z</m>.
    </p>
    <p>
      By our assumption that <m>g(w) = g(z)</m>, as <m>g</m> is a bijection, in particular one-to-one, <m>w=z</m>. Hence 
      <m>f(x) = f(y)</m>. Since <m>f</m> is a bijection, in particular one-to-one, <m>x=y</m>.
    </p>
    <p>
      <alert>[Onto]</alert> (WTS: Rng<m>(g\circ f) = C</m>)
    </p>
    <p>
      <alert>[<m>\subset</m>]</alert>
    </p>
    <p>
      Let <m>y\in \text{ Rng}(g\circ f)</m>. By definition of range, <m>y\in C</m>. Thus, Rng<m>(g\circ f) \subset C</m>.
    </p>
    <p>
      <alert>[<m>\subset</m>]</alert>
    </p>
    <p>
      Let <m>y\in C</m>. Thus by our assumption that <m>g</m> is a bijection, specifically surjective, we can find <m>w\in B</m>
      such that <m>g(w) = y</m>.
    </p>
    <p>
      Thus by assumption that <m>f</m> is a bijection, specifically surjective, we can find <m>x\in A</m> such that <m>f(x) = w</m>.
      Thus by definition of composition, <m>g\circ f(x) =  y</m>. Hence, <m>y\in \text{ Rng}(g\circ f)</m>. Thus
      <m>C \subset \text{ Rng}(g\circ f)</m>.
    </p>
    <p>
      Thus, Rng<m>(g\circ f) = C</m>
    </p>
    <p>
      Thus, <m>g\circ f: A \rightarrow C</m> is a bijection. 
    </p>
  </proof>
  
  <theorem xml:id="thm-10-4-4">
    <statement>
      <p>
        <m>f^{-1}</m> is a function from Rng(<m>f</m>) to <m>A</m> if and only if <m>f</m> is one-to-one.
      </p>
    </statement>
  </theorem>

  <proof>
    <p>
      [<m>\impliedby</m>] (If <m>f</m> is one-to-one, then <m>f^{-1}</m> is a function from Rng(<m>f</m>) to <m>A</m>.)
    </p>
    <p>
      1.) Assume <m>f</m> is one-to-one. We want to show that Dom(<m>f^{-1})=</m>Rng(<m>f</m>). This proof is in section 10.6.1.
    </p>
    <p>
      2.) Let <m>x \in B</m> and <m>y, z \in A</m> such that <m>f^{-1}(x)=y</m> and <m>f^{-1}(x)=z</m>. By definition of inverse, <m>f(y)=x</m>
      and <m>f(z)=x</m>. Thus, by our assumption, <m>y=z</m>.
    </p>
    <p>
      [<m>\implies</m>]
    </p>
    <p>
      Assume <m>f^{-1}</m> is a function from Rng(<m>f</m>) to <m>A</m>, that is, <m>(f: \text{ Rng}(f) \rightarrow A)</m>
    </p>
    <p>
      Let <m>x,y \in A</m> such that <m>f(x)=f(y)</m>. Name this element <m>(f(x)=f(y))</m> something, say, <m>w</m>. By definition of inverse, <m>f^{-1}(w)=x</m>
      and <m>f^{-1}(w)=y</m>. Thus, by our assumption, <m>x=y</m>.
    </p>
  </proof>

  <theorem>
    <statement>
      <p>
        Let <m>f: A \rightarrow B, C</m> and <m>D</m> be subsets of <m>A</m>, and <m>E</m> and <m>F</m> be subsets of <m>B</m>. Since <m>C</m> is a subset,
        <m>f(C) = </m> the image of <m>C</m>.
      </p>
      <ol marker="(a)">
        <li>
          <p>
            <m>f(C\cap D) \subset f(C) \cap f(D)</m>
          </p>
        </li>
        <li>
          <p>
            <m>f^{-1}(E \cap F) = f^{-1}(E) \cap f^{-1}(F)</m>
          </p>
        </li>
      </ol>
    </statement>
  </theorem>

  <proof>
    <p>
      (a) <m>f(C\cap D) \subset f(C) \cap f(D)</m>
    </p>
    <p>
      Let <m>x\in f(C\cap D)</m>.
    </p>
  </proof>
  
</section>
</section>