<?xml version="1.0" encoding="UTF-8"?>

<section xml:id="sec-1-4" xmlns:xi="http://www.w3.org/2001/XInclude">
<title>Exercises</title>
<ol> 
<li>
    <p>Write truth tables for the following:</p>
    <ol>
        
        <li><m>P \iff Q</m></li>
      
        <li><m>(P \implies Q)\vee Q</m></li>
        <li><m>(P\wedge R)\implies Q</m></li>
        <li><m>(\sim Q)\implies Q</m></li>
        <li><m>P\vee (\sim P)</m></li>
        <li><m>\sim (P\wedge Q)</m></li>
        <li><m>(\sim P)\vee (\sim Q)</m></li>
        <li><m>(\sim P)\implies (R\wedge Q)</m></li>
    </ol>
</li>
<li>
    <p>
        Show the remaining laws are from <xref ref="thm-logic-laws"/> are true, using truth tables.
    </p>
</li>
<li>
    <p>Use a truth table to show whether the following are or are not equivalent:</p>
        <ol>
            <li><m>[P\implies ((\sim Q)\wedge R)]</m>, <m>[(P\implies (\sim Q))\vee (P\implies R)]</m></li>
            <li><m>[((\sim P)\vee Q)\implies R]</m>, <m>[((\sim R)\implies P)\wedge (Q\implies R)]</m></li>
            <li><m>[(P\wedge (\sim Q)) \implies R]</m>, <m>[P\implies (Q\vee R)]</m></li>
            <li><m>[(P\implies Q)\wedge (\sim R)]</m>, <m>[(R\vee P)\implies ((\sim R)\wedge Q)]</m></li>
        </ol>
    </li>
    <li>
    <p>Turn the first statement into the second one. Show your steps and state which equivalence rule from 1.3.2 you used to get there.</p>
        <ol>
            <li><m>[P\implies ((\sim Q)\wedge R)]\equiv [(P\implies (\sim Q))\wedge (P\implies R)]</m></li>
            <li><m>[((\sim P)\vee Q)\implies R]\equiv [((\sim R)\implies P)\wedge (Q\implies R)]</m></li>
            <li><m>[(P\wedge (\sim Q))\implies R]\equiv [P\implies (Q\vee R)]</m></li>
            <li><m>[(P\implies Q)\wedge (\sim R)]\equiv [(R\vee P)\implies ((\sim R)\wedge Q)]</m></li>
        </ol>
    </li>
    <li>
        <p>
            Consider the statement <me>\exists x \in \mathbb{R} \text{ such that } x^3 = 3.</me> 
            Which of the following are also ways of saying 
            this statement? (identify all that apply)
            <ol>
                <li>There is at least one real number whose cube is 3.</li>
                <li>The cube of each real number is 3.</li>
                <li>Some real numbers have cube 3.</li>
                <li>The number <m>x</m> has cube 3, for some real number <m>x</m>.</li>
                <li>If <m>x</m> is a real number, then <m>x^3=3</m>.</li>
                <li>Some real number has cube 3.</li>
            </ol>
        </p>
    </li>
    <li>
        <p>Consider the statement <me>\forall n \in \mathbb{Z} \text{ if } n+1 \text{ is even then } n \text{ is odd.}</me> 
            Which of the following are also
            ways of saying this statement? (identify all that apply)
            <ol>
                <li>If the sum of an integer and one is even, then that integer is odd.</li>
                <li>All integers are even once you add one and are odd.</li>
                <li>Given any integer which once adding one is even, that integer must be odd.</li>
                <li>For all integers, there are some which you add one then it is even.</li>
                <li>Any integer which is even once adding one is odd.</li>
                <li>All odd integers are even once adding one.</li>
            </ol>
        </p>
    </li>
    <li>
        <p>
            Translate the following English statements into symbolic sentences with quantifiers. The universe for each is given in the parenthetical.
        </p>
        <ol>
            <li>
                <p>
                    Not all math students are hardworking. (<m>\mathcal{U}=</m>all students)
                </p>
            </li>
            <li>
                <p>
                    All math students are not hardworking. (<m>\mathcal{U}=</m>all students)
                </p>
            </li>
            <li>
                <p>
                    There is a smallest positive integer (<m>\mathcal{U}=\mathbb{R}</m>)
                </p>
            </li>
            <li>
                <p>
                    Some people are happy and some people are not happy. (<m>\mathcal{U}=</m>all people)
                </p>
            </li>
            <li>
                <p>
                    No one loves everybody
                </p>
            </li>
        </ol>
    </li>
   
    
   
    
    <li>
        <p>Rewrite the statement in English without using the symbols 
            <m>\forall</m> or <m>\exists</m>. Express your answer as simply as possible. 
            Then write a negation for the statement. Determine which statement is true, the original or the negation.
            <ol>
                <li><m>\exists \text{ a book } b, \forall \text{ people } p, p \text{ has read } b.</m></li>
                <li><m>\forall \text{ odd integers } n, \exists \text{ an integer } k \text{ such that } n=2k+1</m>.</li>
                <li><m>\forall r \in \mathbb{Q}, \exists \text{ integers } a \text{ and } b \text{ such that } r=a/b</m>.</li>
              
            </ol>
        </p>
    </li>
    <li>
        <p>Rewrite the statement formally using quantifiers and variables. Write the negation of the statement.
            <ol>
                <li>Everybody believes somebody.</li>
                <li>Somebody believes everybody.</li>
                <li>Any even integer equals some other integer plus 1.</li>
                <li>The number of rows in any truth-table is <m>2^n</m> for some integer <m>n</m>.</li>
                
            </ol>
        </p>
    </li>
    
    
</ol>
</section>