<?xml version="1.0" encoding="UTF-8"?>

<section xml:id="subsec-2-4-3-logic-algebra" xmlns:xi="http://www.w3.org/2001/XInclude">
    <title>The Algebra of Logic</title>
    
    <p>
        Now that we have established the laws in <xref ref="thm-logic-laws"/>, we have a new way to prove two
        propositional forms are equivalent. It is what I playfully refer to as the algebra of logic. 
    </p>
    <example>
    <p>
        For a first example of this, let's see a proof that <me>[(P\vee Q)\implies R]\equiv [(P\implies R)\wedge (Q\implies R)]</me>
    </p>
   <proof>
   
    <md>
        <mrow>(P\vee Q)\implies R\amp \equiv [\sim (P\vee Q)]\vee R \text{ (Rob's Law)}</mrow>
        <mrow>\amp \equiv [(\sim P)\wedge (\sim Q)]\vee R \text{ (De Morgan's)}</mrow>
        <mrow>\amp \equiv R \vee [(\sim P)\wedge (\sim Q)] \text{ (commutativity)}</mrow>
        <mrow>\amp \equiv [R \vee (\sim P)]\wedge [R\vee (\sim Q)] \text{ (distributivity)}</mrow>
        <mrow>\amp \equiv [(\sim P)\vee R]\wedge [(\sim Q)\vee R] \text{ (commutativity)}</mrow>
        <mrow>\amp \equiv [(P\implies R)\wedge (Q\implies R)] \text{ (Rob's Law)}</mrow>
    </md>
</proof>
</example>
<p>
    There are many examples for you to try in this chapter's exercises, but we will leave you with one more example.</p> 
  <example>
    <p> <me>[P\implies(Q\implies R)]\equiv[(P\wedge Q)\implies R]</me>
</p>
<proof>
   
    <md>
        <mrow>[P\implies (Q\implies R)\amp \equiv [(\sim P)\vee (Q\implies R)] \text{ (Rob's Law)}</mrow>
        <mrow>\amp \equiv [(\sim P)\vee ((\sim Q)\vee R)] \text{ (Rob's Law)}</mrow>
        <mrow>\amp \equiv [(\sim P)\vee(\sim Q)]\vee R \text{ (associativity)}</mrow>
        <mrow>\amp \equiv \sim(P\wedge Q)\vee R \text{ (DeMorgan's)}</mrow>
        <mrow>\amp \equiv [(P\wedge Q)\implies R] \text{ (Rob's Law)}</mrow>
    </md>
</proof>
</example>
</section>